library/data/rbtree/contains.lean
@@ -1,0 +1,85 @@
+/-
+Copyright (c) 2017 Microsoft Corporation. All rights reserved.
+Released under Apache 2.0 license as described in the file LICENSE.
+Authors: Leonardo de Moura
+-/
+import data.rbtree.basic
+universe u
+
+/- TODO(Leo): remove after we cleanup stdlib simp lemmas -/
+local attribute [-simp] or.comm or.left_comm or.assoc and.comm and.left_comm and.assoc
+
+namespace rbnode
+variables {α : Type u}
+
+@[elab_simple]
+lemma contains.induction {p : rbnode α → Prop} (lt) [decidable_rel lt]
+   (t x)
+   (h₁ : p leaf)
+   (h₂ : ∀ l y r (h : cmp_using lt x y = ordering.lt) (ih : p l), p (red_node l y r))
+   (h₃ : ∀ l y r (h : cmp_using lt x y = ordering.eq),            p (red_node l y r))
+   (h₄ : ∀ l y r (h : cmp_using lt x y = ordering.gt) (ih : p r), p (red_node l y r))
+   (h₅ : ∀ l y r (h : cmp_using lt x y = ordering.lt) (ih : p l), p (black_node l y r))
+   (h₆ : ∀ l y r (h : cmp_using lt x y = ordering.eq),            p (black_node l y r))
+   (h₇ : ∀ l y r (h : cmp_using lt x y = ordering.gt) (ih : p r), p (black_node l y r))
+   : p t :=
+begin
+  induction t,
+  case leaf {assumption},
+  case red_node l y r {
+     generalize h : cmp_using lt x y = c,
+     cases c,
+     case ordering.lt { apply h₂, assumption, assumption },
+     case ordering.eq { apply h₃, assumption },
+     case ordering.gt { apply h₄, assumption, assumption },
+  },
+  case black_node l y r {
+     generalize h : cmp_using lt x y = c,
+     cases c,
+     case ordering.lt { apply h₅, assumption, assumption },
+     case ordering.eq { apply h₆, assumption },
+     case ordering.gt { apply h₇, assumption, assumption },
+  }
+end
+
+lemma contains_correct {t : rbnode α} {lt x} [decidable_rel lt] [is_strict_weak_order α lt] : ∀ {lo hi} (hs : is_searchable lt t lo hi), mem lt x t ↔ contains lt t x = tt :=
+begin
+  apply contains.induction lt t x; intros; simp only [mem, contains, *],
+  { simp },
+  twice { -- red and black cases are identical
+    {
+      cases hs,
+      apply iff.intro,
+      {
+        intro hm, blast_disjs,
+        { exact iff.mp (ih hs₁) hm },
+        { simp at h, cases hm, contradiction },
+        {
+          have hyx : lift lt (some y) (some x) := (range hs₂ hm).1,
+          simp [lift] at hyx,
+          have hxy : lt x y, { simp [cmp_using] at h, assumption },
+          exact absurd (trans_of lt hxy hyx) (irrefl_of lt x)
+        }
+      },
+      { intro hc, left, exact iff.mpr (ih hs₁) hc },
+    },
+    { simp at h, simp [h] },
+    {
+      cases hs,
+      apply iff.intro,
+      {
+        intro hm, blast_disjs,
+        {
+          have hxy : lift lt (some x) (some y) := (range hs₁ hm).2,
+          simp [lift] at hxy,
+          have hyx : lt y x, { simp [cmp_using] at h, exact h.2 },
+          exact absurd (trans_of lt hxy hyx) (irrefl_of lt x)
+        },
+        { simp at h, cases hm, contradiction },
+        { exact iff.mp (ih hs₂) hm }
+      },
+      { intro hc, right, right, exact iff.mpr (ih hs₂) hc },
+    } }
+end
+
+end rbnode
