library/data/rbtree/default.lean
@@ -3,4 +3,4 @@ Copyright (c) 2017 Microsoft Corporation. All rights reserved.
 Released under Apache 2.0 license as described in the file LICENSE.
 Authors: Leonardo de Moura
 -/
-import data.rbtree.lemmas
+import data.rbtree.main
