library/data/rbtree/main.lean
@@ -1,0 +1,81 @@
+/-
+Copyright (c) 2017 Microsoft Corporation. All rights reserved.
+Released under Apache 2.0 license as described in the file LICENSE.
+Authors: Leonardo de Moura
+-/
+import data.rbtree.contains data.rbtree.insert data.rbtree.min_max
+universes u
+
+/- TODO(Leo): remove after we cleanup stdlib simp lemmas -/
+local attribute [-simp] or.comm or.left_comm or.assoc and.comm and.left_comm and.assoc
+
+namespace rbnode
+variables {α : Type u} {lt : α → α → Prop}
+
+lemma is_searchable_of_well_formed {t : rbnode α} [is_strict_weak_order α lt] : t.well_formed lt → is_searchable lt t none none :=
+begin
+  intro h, induction h,
+  { constructor, simp [lift] },
+  { subst n', apply is_searchable_insert, assumption }
+end
+
+end rbnode
+
+namespace rbtree
+variables {α : Type u} {lt : α → α → Prop}
+
+lemma not_mem_mk_rbtree : ∀ (a : α), a ∉ mk_rbtree α lt :=
+by simp [has_mem.mem, rbtree.mem, rbnode.mem, mk_rbtree]
+
+variables [decidable_rel lt]
+
+lemma contains_correct [is_strict_weak_order α lt] (a : α) (t : rbtree α lt) : a ∈ t ↔ (t.contains a = tt) :=
+begin cases t, apply rbnode.contains_correct, apply rbnode.is_searchable_of_well_formed, assumption end
+
+lemma mem_insert_of_incomp {a b : α} (t : rbtree α lt) : (¬ lt a b ∧ ¬ lt b a) → a ∈ t.insert b :=
+begin cases t, apply rbnode.mem_insert_of_incomp end
+
+lemma mem_insert [is_irrefl α lt] : ∀ (a : α) (t : rbtree α lt), a ∈ t.insert a :=
+begin intros, apply mem_insert_of_incomp, split; apply irrefl_of lt end
+
+lemma mem_insert_of_equiv {a b : α} (t : rbtree α lt) : a ≈[lt] b → a ∈ t.insert b :=
+begin cases t, apply rbnode.mem_insert_of_incomp end
+
+lemma mem_insert_of_mem [is_strict_weak_order α lt] {a : α} {t : rbtree α lt} (b : α) : a ∈ t → a ∈ t.insert b :=
+begin cases t, apply rbnode.mem_insert_of_mem end
+
+lemma equiv_or_mem_of_mem_insert [is_strict_weak_order α lt] {a b : α} {t : rbtree α lt} : a ∈ t.insert b → a ≈[lt] b ∨ a ∈ t :=
+begin cases t, apply rbnode.equiv_or_mem_of_mem_insert end
+
+lemma incomp_or_mem_of_mem_ins [is_strict_weak_order α lt] {a b : α} {t : rbtree α lt} : a ∈ t.insert b → (¬ lt a b ∧ ¬ lt b a) ∨ a ∈ t :=
+equiv_or_mem_of_mem_insert
+
+lemma eq_or_mem_of_mem_ins [is_strict_total_order α lt] {a b : α} {t : rbtree α lt} : a ∈ t.insert b → a = b ∨ a ∈ t :=
+begin
+  intro h,
+  have h₁ := incomp_or_mem_of_mem_ins h,
+  have := trichotomous_of lt a b,
+  blast_disjs,
+  any_goals { simp [*] },
+  all_goals { cases h₁, contradiction }
+end
+
+lemma mem_of_min_eq [is_irrefl α lt] {a : α} {t : rbtree α lt} : t.min = some a → a ∈ t :=
+begin cases t, apply rbnode.mem_of_min_eq end
+
+lemma mem_of_max_eq [is_irrefl α lt] {a : α} {t : rbtree α lt} : t.max = some a → a ∈ t :=
+begin cases t, apply rbnode.mem_of_max_eq end
+
+lemma eq_leaf_of_min_eq_none [is_strict_weak_order α lt] {t : rbtree α lt} : t.min = none → t = mk_rbtree α lt :=
+begin cases t, intro h, congr, apply rbnode.eq_leaf_of_min_eq_none h end
+
+lemma eq_leaf_of_max_eq_none [is_strict_weak_order α lt] {t : rbtree α lt} : t.max = none → t = mk_rbtree α lt :=
+begin cases t, intro h, congr, apply rbnode.eq_leaf_of_max_eq_none h end
+
+lemma min_is_minimal [is_strict_weak_order α lt] {a : α} {t : rbtree α lt} : t.min = some a → ∀ {b}, b ∈ t → a ≈[lt] b ∨ lt a b :=
+begin cases t, apply rbnode.min_is_minimal, apply rbnode.is_searchable_of_well_formed, assumption end
+
+lemma max_is_maximal [is_strict_weak_order α lt] {a : α} {t : rbtree α lt} : t.max = some a → ∀ {b}, b ∈ t → a ≈[lt] b ∨ lt b a :=
+begin cases t, apply rbnode.max_is_maximal, apply rbnode.is_searchable_of_well_formed, assumption end
+
+end rbtree
