library/data/rbtree/min_max.lean
@@ -1,0 +1,105 @@
+/-
+Copyright (c) 2017 Microsoft Corporation. All rights reserved.
+Released under Apache 2.0 license as described in the file LICENSE.
+Authors: Leonardo de Moura
+-/
+import data.rbtree.basic
+universe u
+
+/- TODO(Leo): remove after we cleanup stdlib simp lemmas -/
+local attribute [-simp] or.comm or.left_comm or.assoc and.comm and.left_comm and.assoc
+
+namespace rbnode
+variables {α : Type u} {lt : α → α → Prop}
+
+lemma mem_of_min_eq (lt : α → α → Prop) [is_irrefl α lt] {a : α} {t : rbnode α} : t.min = some a → mem lt a t :=
+begin
+   induction t,
+   { intros, contradiction },
+   all_goals {
+     cases lchild; simp [rbnode.min]; intro h,
+     { injection h, subst val, simp [mem, irrefl_of lt a] },
+     all_goals { rw [mem], simp [ih_1 h] } }
+end
+
+lemma mem_of_max_eq (lt : α → α → Prop) [is_irrefl α lt] {a : α} {t : rbnode α} : t.max = some a → mem lt a t :=
+begin
+   induction t,
+   { intros, contradiction },
+   all_goals {
+     cases rchild; simp [rbnode.max]; intro h,
+     { injection h, subst val, simp [mem, irrefl_of lt a] },
+     all_goals { rw [mem], simp [ih_2 h] } }
+end
+
+variables [decidable_rel lt] [is_strict_weak_order α lt]
+
+lemma eq_leaf_of_min_eq_none {t : rbnode α} : t.min = none → t = leaf :=
+begin
+  induction t,
+  { intros, refl },
+  all_goals {
+    cases lchild; simp [rbnode.min]; intro h,
+    { contradiction },
+    all_goals { have := ih_1 h, contradiction } }
+end
+
+lemma eq_leaf_of_max_eq_none {t : rbnode α} : t.max = none → t = leaf :=
+begin
+  induction t,
+  { intros, refl },
+  all_goals {
+    cases rchild; simp [rbnode.max]; intro h,
+    { contradiction },
+    all_goals { have := ih_2 h, contradiction } }
+end
+
+lemma min_is_minimal {a : α} {t : rbnode α} : ∀ {lo hi}, is_searchable lt t lo hi → t.min = some a → ∀ {b}, mem lt b t → a ≈[lt] b ∨ lt a b :=
+begin
+  induction t,
+  { simp [strict_weak_order.equiv], intros _ _ hs hmin b, contradiction },
+  all_goals {
+    cases lchild; intros lo hi hs hmin b hmem,
+    { simp [rbnode.min] at hmin, injection hmin, subst val,
+      simp [mem] at hmem, cases hmem with heqv hmem,
+      { left, exact heqv.swap },
+      { have := lt_of_mem_right hs (by constructor) hmem,
+        right, assumption } },
+    all_goals {
+      cases hs, simp [rbnode.min] at hmin,
+      rw [mem] at hmem, blast_disjs,
+      { exact ih_1 hs₁ hmin hmem },
+      { have hmm       := mem_of_min_eq lt hmin,
+        have a_lt_val  := lt_of_mem_left hs (by constructor) hmm,
+        have a_lt_b    := lt_of_lt_of_incomp a_lt_val hmem.swap,
+        right, assumption },
+      { have hmm       := mem_of_min_eq lt hmin,
+        have a_lt_b    := lt_of_mem_left_right hs (by constructor) hmm hmem,
+        right, assumption } } }
+end
+
+lemma max_is_maximal {a : α} {t : rbnode α} : ∀ {lo hi}, is_searchable lt t lo hi → t.max = some a → ∀ {b}, mem lt b t → a ≈[lt] b ∨ lt b a :=
+begin
+  induction t,
+  { simp [strict_weak_order.equiv], intros _ _ hs hmax b, contradiction },
+  all_goals {
+    cases rchild; intros lo hi hs hmax b hmem,
+    { simp [rbnode.max] at hmax, injection hmax, subst val,
+      simp [mem] at hmem, cases hmem with hmem heqv,
+      { have := lt_of_mem_left hs (by constructor) hmem,
+        right, assumption },
+      { left, exact heqv.swap } },
+    all_goals {
+      cases hs, simp [rbnode.max] at hmax,
+      rw [mem] at hmem, blast_disjs,
+      { have hmm       := mem_of_max_eq lt hmax,
+        have a_lt_b    := lt_of_mem_left_right hs (by constructor) hmem hmm,
+        right, assumption },
+      { have hmm       := mem_of_max_eq lt hmax,
+        have val_lt_a  := lt_of_mem_right hs (by constructor) hmm,
+        have a_lt_b    := lt_of_incomp_of_lt hmem val_lt_a,
+        right, assumption },
+      { exact ih_2 hs₂ hmax hmem } } }
+end
+
+end rbnode
